finish DeriveContextInput

src/cddl/test/dpe/CDDLTest.DPE.DeriveContextInput.fst
@@ -37,51 +37,49 @@ let is_engine_record_core
   rel_evercddl_bytes e.l0_binary_hash wx._x3 **
   rel_evercddl_bytes e.l0_image_auth_pubkey wx._x4
 
-let is_engine_record (e:engine_record) (se:spec_engine_record) : slprop =
+[@@pulse_unfold]
+let is_engine_record (e:engine_record) (se:spec_engine_record) res : slprop =
   is_engine_record_core e se **
-  Trade.trade (is_engine_record_core e se) (rel_evercddl_derive_context_engine_record e se)
+  Trade.trade (is_engine_record_core e se) res
 
 
 ghost
 fn extract_derive_context_engine_record x (w:erased _)
 requires rel_evercddl_derive_context_engine_record x w
-ensures is_engine_record x w
+ensures is_engine_record x w (rel_evercddl_derive_context_engine_record x w)
 {
   Trade.rewrite_with_trade 
     (rel_evercddl_derive_context_engine_record x w)
     (is_engine_record_core x w);
-  fold (is_engine_record x w);
 }
 
 let device_id_csr_ingredients = evercddl_device_id_csr_ingredients_pretty
 let spec_device_id_csr_ingredients = spect_evercddl_device_id_csr_ingredients_pretty
-[@@pulse_unfold]
 let is_device_id_csr_ingredients_core (e:device_id_csr_ingredients) (se:spec_device_id_csr_ingredients) : slprop =
     rel_evercddl_nint e.ku se._x0 **
     rel_evercddl_nint e.version se._x1 **
     rel_evercddl_tstr e.s_common se._x2 **
     rel_evercddl_tstr e.s_org se._x3 **
     rel_evercddl_tstr e.s_country se._x4
-let is_device_id_csr_ingredients (e:device_id_csr_ingredients) (se:spec_device_id_csr_ingredients) : slprop =
+
+[@@pulse_unfold]
+let is_device_id_csr_ingredients (e:device_id_csr_ingredients) (se:spec_device_id_csr_ingredients) res : slprop =
     is_device_id_csr_ingredients_core e se **
-    Trade.trade (is_device_id_csr_ingredients_core e se) (rel_evercddl_device_id_csr_ingredients e se)
+    Trade.trade (is_device_id_csr_ingredients_core e se) res
     
 ghost 
 fn extract_device_id_csr_ingredients x (w:erased _)
 requires rel_evercddl_device_id_csr_ingredients x w
-ensures is_device_id_csr_ingredients x w
+ensures is_device_id_csr_ingredients x w (rel_evercddl_device_id_csr_ingredients x w)
 {
   Trade.rewrite_with_trade 
     (rel_evercddl_device_id_csr_ingredients x w)
     (is_device_id_csr_ingredients_core x w);
-  fold (is_device_id_csr_ingredients x w);
 }
 
 let alias_key_crt_ingredients = evercddl_alias_key_crt_ingredients_pretty
 let spec_alias_key_crt_ingredients = spect_evercddl_alias_key_crt_ingredients_pretty
 
-[@@pulse_unfold]
-unfold
 let is_alias_key_crt_ingredients_core (e:alias_key_crt_ingredients) (s:spec_alias_key_crt_ingredients) =
   rel_evercddl_nint e.version s._x0 **
   rel_evercddl_bytes e.serial_78umber s._x1 **
@@ -95,24 +93,23 @@ let is_alias_key_crt_ingredients_core (e:alias_key_crt_ingredients) (s:spec_alia
   rel_evercddl_nint e.ku s._x9 **
   rel_evercddl_nint e.l0_version s._x10
 
-let is_alias_key_crt_ingredients (e:alias_key_crt_ingredients) (s:spec_alias_key_crt_ingredients) : slprop =
+[@@pulse_unfold]
+let is_alias_key_crt_ingredients (e:alias_key_crt_ingredients) (s:spec_alias_key_crt_ingredients) (res:slprop) : slprop =
   is_alias_key_crt_ingredients_core e s **
-  Trade.trade (is_alias_key_crt_ingredients_core e s) (rel_evercddl_alias_key_crt_ingredients e s)
+  Trade.trade (is_alias_key_crt_ingredients_core e s) res
 
 ghost
 fn extract_alias_key_crt_ingredients x (w:erased _)
 requires rel_evercddl_alias_key_crt_ingredients x w
-ensures is_alias_key_crt_ingredients x w
+ensures is_alias_key_crt_ingredients x w (rel_evercddl_alias_key_crt_ingredients x w)
 {
   Trade.rewrite_with_trade 
     (rel_evercddl_alias_key_crt_ingredients x w)
     (is_alias_key_crt_ingredients_core x w);
-  fold (is_alias_key_crt_ingredients x w);
 }
 
 let l0_record = evercddl_derive_context_l0_record_pretty
 let spec_l0_record = spect_evercddl_derive_context_l0_record_pretty
-[@@pulse_unfold]
 let is_l0_record_core (e:l0_record) (wx:spec_l0_record) : slprop =
   rel_evercddl_bytes e.fwid wx._x0 **
   rel_evercddl_bytes e.device_id_label wx._x1 **
@@ -120,111 +117,80 @@ let is_l0_record_core (e:l0_record) (wx:spec_l0_record) : slprop =
   is_device_id_csr_ingredients_core e.device_id_csr_ingredients wx._x3 **
   is_alias_key_crt_ingredients_core e.alias_key_crt_ingredients wx._x4
 
-let is_l0_record (e:l0_record) (se:spec_l0_record) : slprop =
+[@@pulse_unfold]
+let is_l0_record (e:l0_record) (se:spec_l0_record) res : slprop =
   is_l0_record_core e se **
-  Trade.trade (is_l0_record_core e se) (rel_evercddl_derive_context_l0_record e se)
+  Trade.trade (is_l0_record_core e se) res
 
 ghost
 fn extract_derive_context_l0_record x (w:erased _)
 requires rel_evercddl_derive_context_l0_record x w
-ensures is_l0_record x w
+ensures is_l0_record x w (rel_evercddl_derive_context_l0_record x w)
 {
   Trade.rewrite_with_trade 
     (rel_evercddl_derive_context_l0_record x w)
     (is_l0_record_core x w);
-  fold (is_l0_record x w);
 }
 
 let is_derive_context_input_args_data
     (e:either engine_record l0_record) 
     (res:either spec_engine_record spec_l0_record)
+    (k:slprop)
 : slprop
 = match e, res with
   | Inl er, Inl s_er ->
-    is_engine_record er s_er **
-    Trade.trade 
-      (is_engine_record er s_er) 
-      (rel_evercddl_derive_context_input_args_data 
-        (evercddl_derive_context_input_args_data_pretty_right e)
-        (spect_evercddl_derive_context_input_args_data_pretty_right res))
+    is_engine_record er s_er k 
   | Inr l0, Inr s_l0 ->
-    is_l0_record l0 s_l0 **
-    Trade.trade 
-      (is_l0_record l0 s_l0) 
-      (rel_evercddl_derive_context_input_args_data 
-        (evercddl_derive_context_input_args_data_pretty_right e)
-        (spect_evercddl_derive_context_input_args_data_pretty_right res))
+    is_l0_record l0 s_l0 k
   | _ -> pure False
+
+ghost
+fn trans_is_derive_context_input
+    (e:either engine_record l0_record) 
+    (res:either spec_engine_record spec_l0_record)
+    (k k':slprop)
+requires 
+  is_derive_context_input_args_data e res k **
+  Trade.trade k k'
+ensures
+  is_derive_context_input_args_data e res k'
+{
+  unfold (is_derive_context_input_args_data e res k);
+  match e {
+    Inl x -> {
+      match res {
+        Inr _ -> { 
+          assert pure (False);
+          unreachable ()
+        }
+
+        Inl w -> {
+          Trade.trade_compose _ _ k';
+          fold (is_derive_context_input_args_data (Inl x) (Inl w) k');
+        }
+      }
+
+    }
+  
+    Inr x -> {
+      match res {
+        Inl _ -> { 
+          assert pure (False);
+          unreachable ()
+        }
+
+        Inr w -> {
+          Trade.trade_compose _ _ k';
+          fold (is_derive_context_input_args_data (Inr x) (Inr w) k');
+        }
+      }
+
+    }
+  }
+}
 
 [@@pulse_unfold]
 let norm_token = emp
-
-ghost
-fn unfold_is_engine_record_trade x y ()
-requires emp
-ensures
-   Trade.trade
-     (is_engine_record x y)
-     (is_engine_record_core x y **
-        Trade.trade
-          (is_engine_record_core x y)
-          (rel_evercddl_derive_context_engine_record x y))
-{
-  ghost
-  fn aux ()
-  requires emp ** is_engine_record x y
-  ensures 
-       (is_engine_record_core x y **
-        Trade.trade
-          (is_engine_record_core x y)
-          (rel_evercddl_derive_context_engine_record x y))
-  {
-    unfold (is_engine_record x y);
-  };
-  Trade.intro_trade _ _ _ aux;
-}
-
-ghost
-fn trade_take (p p' q r:slprop) 
-requires Trade.trade q r ** Trade.trade p (p' ** Trade.trade p' q)
-ensures Trade.trade p r
-{
-  ghost
-  fn aux ()
-  requires (Trade.trade q r ** Trade.trade p (p' ** Trade.trade p' q)) ** p
-  ensures r
-  {
-    Trade.elim_trade p _;
-    Trade.elim_trade p' _;
-    Trade.elim_trade _ r;
-  };
-  Trade.intro_trade _ _ _ aux;
-}
-
-ghost
-fn unfold_is_l0_record_trade x y ()
-requires emp
-ensures
-   Trade.trade
-     (is_l0_record x y)
-     (is_l0_record_core x y **
-        Trade.trade
-          (is_l0_record_core x y)
-          (rel_evercddl_derive_context_l0_record x y))
-{
-  ghost
-  fn aux ()
-  requires emp ** is_l0_record x y
-  ensures 
-       (is_l0_record_core x y **
-        Trade.trade
-          (is_l0_record_core x y)
-          (rel_evercddl_derive_context_l0_record x y))
-  {
-    unfold (is_l0_record x y);
-  };
-  Trade.intro_trade _ _ _ aux;
-}
 
 ghost
 fn destruct_rel_either_left 
@@ -298,6 +264,7 @@ requires rel_evercddl_derive_context_input_args_data x w
 ensures is_derive_context_input_args_data 
           (evercddl_derive_context_input_args_data_pretty_left x)
           (spect_evercddl_derive_context_input_args_data_pretty_left w)
+          (rel_evercddl_derive_context_input_args_data x w)
 {
   unfold_with_trade (`%rel_evercddl_derive_context_input_args_data) (rel_evercddl_derive_context_input_args_data _ _);
   destruct_rel_fun _ _ _ _ _;
@@ -307,9 +274,8 @@ ensures is_derive_context_input_args_data
     Inl _ -> {
       let _ = destruct_rel_either_left _ _ _ _ _;
       let engine_record = extract_derive_context_engine_record _ _;
-      with xx yy. assert (is_engine_record xx yy);
-      unfold_is_engine_record_trade xx yy ();
-      trade_take (is_engine_record xx yy) _ _ _;
+      with xx yy. assert (is_engine_record_core xx yy);
+      Trade.trade_compose _ _ (rel_evercddl_derive_context_input_args_data x w);
       rewrite each x as (evercddl_derive_context_input_args_data_pretty_right (Inl xx));
       rewrite each w as (spect_evercddl_derive_context_input_args_data_pretty_right (Inl yy));
       fold (is_derive_context_input_args_data (Inl xx) (Inl yy));
@@ -318,9 +284,8 @@ ensures is_derive_context_input_args_data
     Inr l0 -> {
       let _ = destruct_rel_either_right _ _ _ _ _;
       let l0_record = extract_derive_context_l0_record _ _;
-      with xx yy. assert (is_l0_record xx yy);
-      unfold_is_l0_record_trade xx yy ();
-      trade_take (is_l0_record xx yy) _ _ _;
+      with xx yy. assert (is_l0_record_core xx yy);
+      Trade.trade_compose _ _ (rel_evercddl_derive_context_input_args_data x w);
       rewrite each x as (evercddl_derive_context_input_args_data_pretty_right (Inr xx));
       rewrite each w as (spect_evercddl_derive_context_input_args_data_pretty_right (Inr yy));
       fold (is_derive_context_input_args_data (Inr xx) (Inr yy));
@@ -328,49 +293,59 @@ ensures is_derive_context_input_args_data
   }
 }
 
-let is_record_opt (e:option (either engine_record l0_record)) (res:option (either spec_engine_record spec_l0_record)) : slprop =
+let is_record_opt
+      (e:option (either engine_record l0_record)) 
+      (res:option (either spec_engine_record spec_l0_record))
+      k : slprop =
   match e, res with
-  | None, None ->
-    rel_option rel_evercddl_derive_context_input_args_data None None
+  | None, None -> k
   | Some ee, Some eres -> 
-    is_derive_context_input_args_data ee eres **
-    Trade.trade 
-      (is_derive_context_input_args_data ee eres)
-      (rel_option rel_evercddl_derive_context_input_args_data 
-        (Some <| evercddl_derive_context_input_args_data_pretty_right ee)
-        (Some <| spect_evercddl_derive_context_input_args_data_pretty_right eres))
+    is_derive_context_input_args_data ee eres k
   | _, _ -> pure False
+
+ghost
+fn is_record_opt_compose
+    (e:option (either engine_record l0_record)) 
+    (res:option (either spec_engine_record spec_l0_record))
+    k k'
+requires is_record_opt e res k ** Trade.trade k k'
+ensures is_record_opt e res k'
+{
+  unfold (is_record_opt e res k);
+  match e {
+    None -> {
+      match res {
+        None -> {  
+          Trade.elim_trade _ _;
+          fold (is_record_opt None None k');
+        }
+        Some _ -> { 
+          assert pure (False);
+          unreachable ()
+        }
+      }
+    }
+
+    Some e -> {
+      match res {
+        None -> { 
+          assert pure (False);
+          unreachable ()
+        }
+        Some res -> {
+          trans_is_derive_context_input _ _ _ _;
+          fold (is_record_opt (Some e) (Some res) k');
+        }
+      }
+    }
+  }
+}
 
 inline_for_extraction
 let map_opt (x:option 'a) (f:'a -> 'b) : option 'b = 
   match x with
   | None -> None
   | Some v -> Some (f v)
-
-ghost
-fn is_record_opt_trade_compose
-    (e:_)//option (either engine_record l0_record)) 
-    (se:_)//option (either spec_engine_record spec_l0_record))
-    (res:slprop) 
-requires
-  is_record_opt 
-    (map_opt e evercddl_derive_context_input_args_data_pretty_left)
-    (map_opt se spect_evercddl_derive_context_input_args_data_pretty_left) **
-  Trade.trade
-    (rel_option rel_evercddl_derive_context_input_args_data e se)
-    res
-ensures
-  is_record_opt 
-    (map_opt e evercddl_derive_context_input_args_data_pretty_left)
-    (map_opt se spect_evercddl_derive_context_input_args_data_pretty_left) **
-  Trade.trade 
-    (is_record_opt 
-      (map_opt e evercddl_derive_context_input_args_data_pretty_left)
-      (map_opt se spect_evercddl_derive_context_input_args_data_pretty_left))
-    res
-{
-  admit()
-}
 
 
 ghost
@@ -397,6 +372,7 @@ ensures
   is_record_opt 
     (map_opt x evercddl_derive_context_input_args_data_pretty_left)
     (map_opt w spect_evercddl_derive_context_input_args_data_pretty_left)
+    (rel_option rel_evercddl_derive_context_input_args_data x w)
 {
   rel_option_cases _ _ _;
   match x {
@@ -405,10 +381,13 @@ ensures
       fold (is_record_opt None None);
       ()
     }
-    Some x -> { 
+    Some v -> { 
+      rewrite each (Some v) as x;
       destruct_rel_option _ _ _;
-      extract_derive_context_input_args_data
-      admit() 
+      extract_derive_context_input_args_data _ _;
+      trans_is_derive_context_input _ _ _ (rel_option rel_evercddl_derive_context_input_args_data x w);
+      with xx yy k. assert (is_derive_context_input_args_data xx yy k);
+      fold (is_record_opt (Some xx) (Some yy));
     }
   }
 }
@@ -460,11 +439,7 @@ requires rel_evercddl_derive_context_input_args x w
 ensures 
   is_record_opt 
     (map_opt x.intkey6 evercddl_derive_context_input_args_data_pretty_left)
-    (map_opt w._x5 spect_evercddl_derive_context_input_args_data_pretty_left) **
-  Trade.trade
-    (is_record_opt 
-      (map_opt x.intkey6 evercddl_derive_context_input_args_data_pretty_left)
-      (map_opt w._x5 spect_evercddl_derive_context_input_args_data_pretty_left))
+    (map_opt w._x5 spect_evercddl_derive_context_input_args_data_pretty_left) 
     (rel_evercddl_derive_context_input_args x w)
 {
   unfold_with_trade
@@ -486,7 +461,7 @@ ensures
           evercddl_derive_context_input_args_data_pretty)
   as evercddl_derive_context_input_args_data_pretty;
   extract_derive_context_input_args_data_opt _ _;
-  is_record_opt_trade_compose _ _ _;
+  is_record_opt_compose _ _ _ _;
 }
 
 
@@ -504,8 +479,7 @@ ensures (
   | _, false -> pts_to s #p w
   | e, _ -> 
     exists* se.
-      is_record_opt e se **
-      Trade.trade (is_record_opt e se) (pts_to s #p w) **
+      is_record_opt e se (pts_to s #p w) **
       pure (is_input_args_data w se)
   )
 
@@ -521,56 +495,8 @@ ensures (
       unfold validate_and_parse_post;
       extract_derive_context_input_args x _;
       Trade.Util.elim_hyp_r _ _ _;
-      Trade.trade_compose _ _ (pts_to s #p w);
+      is_record_opt_compose _ _ _ _;
       (map_opt x.intkey6 evercddl_derive_context_input_args_data_pretty_left, true)
     }
   }
 }
-
-(*)
-  is_record_opt (e:option (either engine_record l0_record)) (res:option (either spec_engine_record spec_l0_record)) : slprop =
-
-// ensures is_derive_context_input e (rel_evercddl_derive_context_input_args x w)
-{
-  unfold_with_trade
-    (`%rel_evercddl_derive_context_input_args) 
-    (rel_evercddl_derive_context_input_args x w);
-  destruct_rel_fun _ _ _ _ _;
-  Trade.trade_compose _ _ (rel_evercddl_derive_context_input_args x w);
-  fold_last_relation (`%tstr_any) tstr_any;  
-  let rest_12 = fst_pair_concrete _ _ _ _ _;
-  let rest_11 = fst_pair_concrete _ _ _ _ _;
-  let rest_10 = fst_pair_concrete _ _ _ _ _;
-  let rest_9 = fst_pair_concrete _ _ _ _ _;
-  let rest_8 = fst_pair_concrete _ _ _ _ _;
-  let rest_7 = fst_pair_concrete _ _ _ _ _;
-  let rest_6 = fst_pair_concrete _ _ _ _ _;
-  let input_data = snd_pair_concrete _ _ _ _ _;
-  rewrite each  
-    (Tactics.PrettifyType.named "intkey6"
-          evercddl_derive_context_input_args_data_pretty)
-  as evercddl_derive_context_input_args_data_pretty;
-  show_proof_state;
-  // extract_option_derive_context_input_args_data _ _ _;
-}
-
-ghost
-fn trans_is_derive_context_input
-     e res res'
-requires is_derive_context_input e res ** Trade.trade res res'
-ensures is_derive_context_input e res'
-{
-  unfold is_derive_context_input;
-  match e {
-    None -> {
-      Trade.elim_trade _ _;
-      fold (is_derive_context_input None res');
-    }
-    Some e -> {
-      assert (is_derive_context_input_args e res);
-      trans_is_derive_context_input_args e res res';
-      fold (is_derive_context_input (Some e) res');
-    }
-  }
-}
-
